EffectSSA/Semantics/Lemmas.lean
@@ -42,12 +42,57 @@ end Instruction
 namespace Semantics.Environment
 variable {env : Environment τ}
 
+/-! ### Grind lemmas -/
+
 @[simp, grind =]
 theorem get?_snoc_zero : (env.snoc x).get? ⟨0⟩ = pure x := rfl
 
 @[simp, grind =]
 theorem getAs_snoc_zero : (env.snoc ⟨t, x⟩).getAs ⟨0⟩ t = pure x := by
-  simp [getAs, getAs?]; rfl
+  simp [getAs, getAs?]
+
+@[simp, grind =] theorem get?_ofList (env : List τ.Val) :
+  (ofList env).get? x = env[x.toNat]? := by rfl
+
+/-! ### WellTyped lemmas -/
+variable {Γ : Context τ}
+
+/--
+If a context `env` is well-typed w.r.t. a context `Γ`, then `env` has precisely
+as many variables as `Γ` has types.
+-/
+@[grind →] theorem size_eq_of_wellTyped (wt : WellTyped Γ env) : env.size = Γ.size := by
+  rcases env with ⟨env⟩
+  rcases Γ with ⟨Γ⟩
+  simp [WellTyped, getAs?] at wt
+  simp [Environment.size, Context.size]
+  induction Γ generalizing env
+  case nil =>
+    simp only [List.length_nil, List.length_eq_zero_iff]
+    ext i
+    specialize wt ⟨i⟩
+    simp_all
+  case cons t Γ ih =>
+    show env.length = Γ.length + 1
+    cases env
+    case nil =>
+      exfalso; simpa using wt ⟨0⟩ t
+    case cons x env =>
+      suffices env.length = Γ.length by simpa
+      apply ih
+      intro v t
+      specialize wt (v + 1) t
+      grind
+
+@[grind →]
+theorem isSome_get?_of_wellTyped (wt : WellTyped Γ env) :
+    ∀ x, Γ[x]?.isSome → (env.get? x).isSome := by
+  cases env; grind
+
+@[grind <=]
+theorem isSome_get_of_wellTyped {Γ} {env : Environment τ} (wt : WellTyped Γ env) :
+    ∀ x, Γ[x]?.isSome → (env.get x).isSome :=
+  isSome_get?_of_wellTyped wt
 
 end Semantics.Environment
 
@@ -71,3 +116,55 @@ variable {es es' : Trace τ}
     StateT.run (putTrace es) none = pure ((), some es) := rfl
 
 end Instruction
+
+/-!
+## Execution Lemmas
+--------------------------------------------------------------------------------
+-/
+section WellTypedExec
+open Semantics (Environment)
+variable {p : Program τ} {Γ ts}
+
+theorem isSome_exec_of_wellTyped {env : Environment τ}
+    (wt_p : p.WellTyped Γ ts)
+    (wt_env : env.WellTyped Γ) :
+    (p.exec env es).isSome := by
+  rcases wt_p with ⟨Δ, wt_p, h_un, h_ts⟩
+  rcases p with ⟨p, returnVars⟩
+  simp_all only [Program.exec, Program.execM]
+  induction wt_p generalizing env
+  case nil Γ _ h =>
+    subst h
+    simp_all only [InstructionSeq.execM_nil, pure_bind, ExecM.run'_some]
+    rw [mapM_liftM, ExecM.run_liftM, Option.map_eq_map, Option.isSome_map, isSome_mapM_iff]
+    intro x hx
+    have : ∃ (i : _) (hi : i < returnVars.length), returnVars[i] = x := List.mem_iff_getElem.mp hx
+    have : Γ[x]?.isSome := by grind
+    grind
+  case cons x xs ih =>
+    simp_all
+    /-
+    TODO:
+    This requires verification of monadic code, which is going to be a pain.
+    I'll leave this sorry for now, but I want to experiment with building an
+    intrinsically well-typed data-structure on top of the untyped one, and then
+    defining the semantics only for well-typed programs.
+    Or at least, defining intrinsically well-typed exec functions defined in
+    terms of the untyped ones + a lemma like this one.
+    -/
+    sorry
+where
+  mapM_liftM {α β m n} [Monad m] [Monad n] [MonadLiftT m n] [LawfulMonadLiftT m n] [LawfulMonad m] [LawfulMonad n]
+      (xs : List α) (f : α → m β) :
+      (xs.mapM fun x => liftM (n:=n) (f x)) = liftM (xs.mapM f) := by
+    induction xs <;> simp_all
+  isSome_mapM_iff {α β} (xs : List α) (f : α → Option β) :
+      (xs.mapM f).isSome = ∀ x ∈ xs, (f x).isSome := by
+    induction xs
+    case nil => simp
+    case cons x xs ih =>
+      simp only [List.mapM_cons, Option.pure_def, Option.bind_eq_bind, List.mem_cons,
+        forall_eq_or_imp]
+      cases f x
+      · simp_all
+      · cases hfx : (List.mapM f xs) <;> simp_all
